<?xml version="1.0"?>
<rdf:RDF 
    xmlns:rdf="http://www.w3.org/1999/02/22-rdf-syntax-ns#"
    xmlns:rdfs="http://www.w3.org/2000/01/rdf-schema#"
    xmlns:base="http://localhost:82/DiscoveryAPI/">
    
    <rdfs:Class rdf:about="http://localhost:82/DiscoveryAPI/#Device">
        <rdfs:label>Device</rdfs:label>
        <rdfs:comment>A Device is usually a constructed tool</rdfs:comment>
    </rdfs:Class>
    
    <rdfs:Class rdf:about="http://localhost:82/DiscoveryAPI/#Actuator">
        <rdfs:subClassOf rdf:resource="http://localhost:82/DiscoveryAPI/#Device"/>
        <rdfs:label>Actuator</rdfs:label>
        <rdfs:comment>An actuator is a type of motor for moving or controlling a mechanism or system</rdfs:comment>
    </rdfs:Class>
    
    <rdfs:Class rdf:about="http://localhost:82/DiscoveryAPI/#Sensor">
        <rdfs:subClassOf rdf:resource="http://localhost:82/DiscoveryAPI/#Device"/>
        <rdfs:label>Sensor</rdfs:label>
        <rdfs:comment>
            A sensor (also called detector) is a converter that measures a physical quantity and converts it into a signal 
            which can be read by an observer or by an (today mostly electronic) instrument
        </rdfs:comment>
    </rdfs:Class>
    
    <rdfs:Class rdf:about="http://localhost:82/DiscoveryAPI/#Lamp">
        <rdfs:subClassOf rdf:resource="http://localhost:82/DiscoveryAPI/#Actuator"/>
        <rdfs:label>Lamp</rdfs:label>
        <rdfs:comment>Lamp (electrical component), a replaceable component that produces light</rdfs:comment>
    </rdfs:Class>
    
    <rdfs:Class rdf:about="http://localhost:82/DiscoveryAPI/#Switch">
        <rdfs:subClassOf rdf:resource="http://localhost:82/DiscoveryAPI/#Actuator"/>
        <rdfs:label>Switch</rdfs:label>
        <rdfs:comment>
            In electrical engineering, a switch is an electrical component that can break an electrical circuit, 
            interrupting the current or diverting it from one conductor to another
        </rdfs:comment>
    </rdfs:Class>
    
    <rdfs:Class rdf:about="http://localhost:82/DiscoveryAPI/#Buzzer">
        <rdfs:subClassOf rdf:resource="http://localhost:82/DiscoveryAPI/#Actuator"/>
        <rdfs:label>Buzzer</rdfs:label>
        <rdfs:comment>Buzzer (electrical component), output sounds</rdfs:comment>
    </rdfs:Class>
    
    <rdfs:Class rdf:about="http://localhost:82/DiscoveryAPI/#Temperature">
        <rdfs:subClassOf rdf:resource="http://localhost:82/DiscoveryAPI/#Sensor"/>
        <rdfs:label>Temperature</rdfs:label>
        <rdfs:comment>
            A thermometer is a device that measures temperature or 
            temperature gradient using a variety of different principles
        </rdfs:comment>
    </rdfs:Class>
    
    <rdfs:Class rdf:about="http://localhost:82/DiscoveryAPI/#Luminosity">
        <rdfs:subClassOf rdf:resource="http://localhost:82/DiscoveryAPI/#Sensor"/>
        <rdfs:label>Luminosity</rdfs:label>
        <rdfs:comment>
            Luminosity is generally understood as a measurement of brightness, 
            in this case measured by a sensor
        </rdfs:comment>
    </rdfs:Class>
    
</rdf:RDF>